coq/SigmaHCOL/SigmaHCOL.v
@@ -226,29 +226,40 @@ Section SigmaHCOL_Operators.
                (op_family: @SHOperatorFamily i o (S n)): @SHOperatorFamily i o n
       := fun jf => op_family (mkFinNat (lt_n_S (proj2_sig jf))).
 
-    Lemma shrink_op_family_facts
-          (i o k : nat)
-          (op_family : SHOperatorFamily)
-          (facts: ∀ (j : nat) (jc : j < S k),
-              @SHOperator_Facts i o (op_family (mkFinNat jc))):
-      (forall (j : nat) (jc : j < k),
-          @SHOperator_Facts i o ((shrink_op_family op_family) (mkFinNat jc))).
-    Proof.
-      intros j jc.
-      apply facts.
-    Defined.
+    Definition shrink_op_family_up_n
+               {i o n: nat}
+               (d: nat)
+               (op_family: @SHOperatorFamily i o (n+d)): @SHOperatorFamily i o n
+      := fun jf => op_family (mkFinNat
+                             (Plus.plus_lt_compat_r _ _ _ (proj2_sig jf))).
 
-    Lemma shrink_op_family_facts_up
-          (i o k : nat)
+    Definition shrink_op_family_facts
+          {i o k : nat}
           (op_family : SHOperatorFamily)
           (facts: ∀ (j : nat) (jc : j < S k),
               @SHOperator_Facts i o (op_family (mkFinNat jc))):
       (forall (j : nat) (jc : j < k),
-          @SHOperator_Facts i o ((shrink_op_family_up op_family) (mkFinNat jc))).
-    Proof.
-      intros j jc.
-      apply facts.
-    Defined.
+          @SHOperator_Facts i o ((shrink_op_family op_family) (mkFinNat jc)))
+      := fun j jc => facts j (le_S jc).
+
+    Definition shrink_op_family_facts_up
+               {i o k : nat}
+               (op_family : SHOperatorFamily)
+               (facts: ∀ (j : nat) (jc : j < S k),
+                   @SHOperator_Facts i o (op_family (mkFinNat jc))):
+      (forall (j : nat) (jc : j < k),
+          @SHOperator_Facts i o ((shrink_op_family_up op_family) (mkFinNat jc)))
+      := fun j jc => facts (S j) (lt_n_S jc).
+
+    Definition shrink_op_family_facts_up_n
+               {i o k : nat}
+               (d: nat)
+               (op_family : SHOperatorFamily)
+               (facts: ∀ (j : nat) (jc : j < (k+d)),
+                   @SHOperator_Facts i o (op_family (mkFinNat jc))):
+      (forall (j : nat) (jc : j < k),
+          @SHOperator_Facts i o ((shrink_op_family_up_n d op_family) (mkFinNat jc)))
+      := fun j jc => facts (j+d) (Plus.plus_lt_compat_r _ _ _ jc).
 
     Fixpoint family_in_index_set
              {i o n}
